Goratha Dapth

Etst/Subtyping/Utils/ExprExpandsInto.lean
@@ -1,11 +1,9 @@
 
 import Etst.WFC.Ch5_S1_AProofSystem
-import Etst.WFC.Utils.PairExprMono
-import Etst.WFC.Utils.ExprMonoEq
+import Etst.WFC.Utils.InterpretationMono
 import Etst.Subtyping.Utils.ExprClearBvars
 
 namespace Etst
-open PairExpr
 
 
 /-
@@ -17,7 +15,7 @@ open PairExpr
 inductive PairExpr.ExpandsInto
   (dl: PairDl)
 :
-  PairExpr → PairExpr → Type
+  BasicPairExpr → BasicPairExpr → Type
 
 | refl e: ExpandsInto dl e e
 | var (x: Nat)
@@ -28,29 +26,29 @@ inductive PairExpr.ExpandsInto
     (left: ExpandsInto dl l lExp)
     (rite: ExpandsInto dl r rExp)
   :
-    ExpandsInto dl (.pair l r) (.pair lExp rExp)
+    ExpandsInto dl (pair l r) (pair lExp rExp)
 | condSome
     (exp: ExpandsInto dl body bodyExp)
   :
-    ExpandsInto dl (.condSome body) (.condSome bodyExp)
+    ExpandsInto dl (condSome body) (condSome bodyExp)
 | condFull
     (exp: ExpandsInto dl body bodyExp)
   :
-    ExpandsInto dl (.condFull body) (.condFull bodyExp)
+    ExpandsInto dl (condFull body) (condFull bodyExp)
 | un
     (left: ExpandsInto dl l lExp)
     (rite: ExpandsInto dl r rExp)
   :
-    ExpandsInto dl (.un l r) (.un lExp rExp)
+    ExpandsInto dl (un l r) (un lExp rExp)
 | ir
     (left: ExpandsInto dl l lExp)
     (rite: ExpandsInto dl r rExp)
   :
-    ExpandsInto dl (.ir l r) (.ir lExp rExp)
-| cpl
+    ExpandsInto dl (ir l r) (ir lExp rExp)
+| compl
     (exp: ExpandsInto dl body bodyExp)
   :
-    ExpandsInto dl (.cpl body) (.cpl bodyExp)
+    ExpandsInto dl (.compl body) (.compl bodyExp)
 | arbUn
     (exp: ExpandsInto dl body bodyExp)
   :
@@ -66,36 +64,41 @@ namespace PairExpr.ExpandsInto
   def rfl {dl e}: ExpandsInto dl e e :=
     ExpandsInto.refl e
   
+  open BasicExpr in
   def intp_eq_wfm
     (dl: PairDl)
     (bv: List Pair)
   :
-    ExpandsInto dl l r → l.intp bv dl.wfm = r.intp bv dl.wfm
+    ExpandsInto dl left rite →
+    left.triIntp bv dl.wfm = rite.triIntp bv dl.wfm
   
   | .refl _ => _root_.rfl
     | .var x expr =>
       let ih := expr.intp_eq_wfm (bv := bv)
       let eqDef := dl.wfm_eq_def pairSalgebra x
-      let eqClean := clearVars_preserves_interp
-        (dl.getDef x) bv dl.wfm dl.wfm
+      let eqClean :=
+        BasicExpr.clearBvars_preserves_interp
+          (dl.getDef x) bv dl.wfm dl.wfm
       eqDef.trans (Eq.trans eqClean ih)
     | .pair left rite =>
-      eq_pair_of_eq (left.intp_eq_wfm dl bv) (rite.intp_eq_wfm dl bv)
+      eq_triIntp2_pair_of_eq (left.intp_eq_wfm dl bv) (rite.intp_eq_wfm dl bv)
     | .un left rite =>
-      eq_un_of_eq (left.intp_eq_wfm dl bv) (rite.intp_eq_wfm dl bv)
+      eq_triIntp2_un_of_eq (left.intp_eq_wfm dl bv) (rite.intp_eq_wfm dl bv)
         | .ir left rite =>
-      eq_ir_of_eq (left.intp_eq_wfm dl bv) (rite.intp_eq_wfm dl bv)
+      eq_triIntp2_ir_of_eq (left.intp_eq_wfm dl bv) (rite.intp_eq_wfm dl bv)
         | .condSome expr =>
-      eq_condSome_of_eq (expr.intp_eq_wfm dl bv)
+      eq_triIntp2_condSome_of_eq (expr.intp_eq_wfm dl bv)
         | .condFull expr =>
-      eq_condFull_of_eq (expr.intp_eq_wfm dl bv)
-        | .cpl expr =>
-      eq_cpl_of_eq (expr.intp_eq_wfm dl bv)
+      eq_triIntp2_condFull_of_eq (expr.intp_eq_wfm dl bv)
+        | .compl expr =>
+      eq_triIntp2_compl_of_eq dl.wfm dl.wfm (expr.intp_eq_wfm dl bv)
         | .arbUn expr =>
-      eq_arbUn_of_eq (fun dB => expr.intp_eq_wfm dl (dB :: bv))
+      eq_triIntp2_arbUn_of_eq (fun dB => expr.intp_eq_wfm dl (dB :: bv))
         | .arbIr expr =>
-      eq_arbIr_of_eq (fun dB => expr.intp_eq_wfm dl (dB :: bv))
+      eq_triIntp2_arbIr_of_eq (fun dB => expr.intp_eq_wfm dl (dB :: bv))
   
+  open BasicExpr in
+  open SingleLaneExpr in
   def lfpStage_le_std
     (expInto: ExpandsInto dl l r)
     (bv: List Pair)
@@ -103,7 +106,7 @@ namespace PairExpr.ExpandsInto
   :
     let _ := Valuation.ordStdLattice
     let op := operatorC pairSalgebra dl dl.wfm
-    let intpN e bv n := intp2 e bv dl.wfm (op.lfpStage n)
+    let intpN e bv n := e.triIntp2 bv dl.wfm (op.lfpStage n)
     
     intpN l bv n ≤ intpN r bv n
   := by
@@ -121,33 +124,33 @@ namespace PairExpr.ExpandsInto
         let eqNext: intpN defX [] n = op.lfpStage n.succ x :=
           congr (op.lfpStage_apply_eq_succ n) _root_.rfl
         let eqClear: intpN defX [] n = intpN defX.clearBvars bv n :=
-          clearVars_preserves_interp (salg := pairSalgebra) _ _ _ _
+          clearBvars_preserves_interp (salg := pairSalgebra) _ _ _ _
         
         eqClear ▸ eqNext ▸ op.lfpStage_mono (Order.le_succ n) x
       leNextStage.trans ih
     | pair left rite =>
       let leLeft := left.lfpStage_le_std bv n
       let leRite := rite.lfpStage_le_std bv n
-      intp_mono_std_pair leLeft leRite
+      triIntp2_mono_std_pair leLeft leRite
     | un left rite =>
       let leLeft := left.lfpStage_le_std bv n
       let leRite := rite.lfpStage_le_std bv n
-      intp_mono_std_un leLeft leRite
+      triIntp2_mono_std_un leLeft leRite
     | ir left rite =>
       let leLeft := left.lfpStage_le_std bv n
       let leRite := rite.lfpStage_le_std bv n
-      intp_mono_std_ir leLeft leRite
+      triIntp2_mono_std_ir leLeft leRite
     | condSome exp =>
-      intp_mono_std_condSome (exp.lfpStage_le_std bv n)
+      triIntp2_mono_std_condSome (exp.lfpStage_le_std bv n)
     | condFull exp =>
-      intp_mono_std_condFull (exp.lfpStage_le_std bv n)
-    | cpl exp =>
+      triIntp2_mono_std_condFull (exp.lfpStage_le_std bv n)
+    | compl exp =>
       let eqBody := exp.intp_eq_wfm dl bv
-      inter_mono_std_cpl (le_of_eq eqBody.symm)
+      triIntp2_mono_std_compl dl.wfm dl.wfm (le_of_eq eqBody.symm)
     | arbUn exp =>
-      inter_mono_std_arbUn (fun dB =>
+      triIntp2_mono_std_arbUn (fun dB =>
         exp.lfpStage_le_std (dB :: bv) n)
     | arbIr exp =>
-      inter_mono_std_arbIr (fun dB =>
+      triIntp2_mono_std_arbIr (fun dB =>
         exp.lfpStage_le_std (dB :: bv) n)
 end PairExpr.ExpandsInto
