Etst/Subtyping/ProofSystem.lean
@@ -14,52 +14,54 @@
   4. A ⊆ t A (coinduction on "B", or precisely on t)
   5. A ⊆ t (A | B)) (combination of 3 and 4, eq to `A ⊆ ~(t' (~A & B'))`)
   
+  TODO emphasize somewhere that induction/coinduction is built with the
+  idea that our inductive structures are in the possible lane, while
+  coinductive structures are in the definite lane.
 -/
 
 import Etst.Subtyping.Utils.ExprExpandsInto
 import Etst.WFC.Ch5_S1_AProofSystem
-import Etst.WFC.Utils.PairExprMono
+import Etst.WFC.Utils.InterpretationMono
 
 namespace Etst
 open PairExpr
 
 
-def IsDefSubset (a b: Set3 Pair) := ∀ ⦃p⦄, p ∈ a.posMem → p ∈ b.defMem
-def IsPosSubset (a b: Set3 Pair) := ∀ ⦃p⦄, p ∈ a.defMem → p ∈ b.posMem
-
-abbrev PairDl.IsDefSubset (dl: PairDl) (a b: PairExpr) :=
-  Etst.IsDefSubset (a.intp [] dl.wfm) (b.intp [] dl.wfm)
-abbrev PairDl.IsPosSubset (dl: PairDl) (a b: PairExpr) :=
-  Etst.IsPosSubset (a.intp [] dl.wfm) (b.intp [] dl.wfm)
+abbrev PairDl.IsDefSubset (dl: PairDl) (a b: SingleLanePairExpr) :=
+  Set.Subset (a.intp [] dl.wfm) (b.intp [] dl.wfm)
+abbrev PairDl.IsPosSubset (dl: PairDl) (a b: SingleLanePairExpr) :=
+  Set.Subset (a.intp [] dl.wfm) (b.intp [] dl.wfm)
 
 
 def Expr.replacePosVars
-  (e: Expr sig)
-  (replacer: Nat → Expr sig)
+  (e: Expr E sig)
+  (replacer: E → Nat → Expr E sig)
 :
-  Expr sig
+  Expr E sig
 :=
   match e with
-  | var x => replacer x
+  | var i x => replacer i x
   | bvar x => .bvar x
   | op o args => op o fun param => (args param).replacePosVars replacer
-  | cpl body => cpl body -- Note: no replacing in complements.
+  | compl body => compl body -- Note: no replacing in complements.
   | arbUn body => arbUn (body.replacePosVars replacer)
   | arbIr body => arbIr (body.replacePosVars replacer)
 
 
+-- Represents an inductive proof of `var .posLane left ⊆ rite`
 structure InductionDescriptor (dl: PairDl) where
   left: Nat
-  rite: PairExpr
+  rite: SingleLanePairExpr
   riteIsClean: rite.IsClean
-  expansion: PairExpr
+  expansion: BasicPairExpr
   expandsInto: ExpandsInto dl (dl.getDef left) expansion
 
+-- Represents a coinductive proof of `left ⊆ var .defLane rite`
 structure CoinductionDescriptor (dl: PairDl) where
-  left: PairExpr
+  left: SingleLanePairExpr
   rite: Nat
   leftIsClean: left.IsClean
-  expansion: PairExpr
+  expansion: BasicPairExpr
   expandsInto: ExpandsInto dl (dl.getDef rite) expansion
 
 abbrev MutIndDescriptor (dl: PairDl) := List (InductionDescriptor dl)
@@ -68,99 +70,108 @@ abbrev MutCoindDescriptor (dl: PairDl) := List (CoinductionDescriptor dl)
 def InductionDescriptor.hypothesis
   (x: Nat)
   (desc: InductionDescriptor dl)
-  (expr: PairExpr)
+  (expr: SingleLanePairExpr)
 :
-  PairExpr
+  SingleLanePairExpr
 :=
-  if desc.left = x then .ir desc.rite expr else expr
+  if desc.left = x then ir desc.rite expr else expr
 
 def CoinductionDescriptor.hypothesis
   (x: Nat)
   (desc: CoinductionDescriptor dl)
-  (expr: PairExpr)
+  (expr: SingleLanePairExpr)
 :
-  PairExpr
+  SingleLanePairExpr
 :=
-  if desc.rite = x then .ir (.cpl desc.left) expr else expr
+  if desc.rite = x then ir (.compl desc.left) expr else expr
 
 def MutIndDescriptor.hypothesis
   (desc: MutIndDescriptor dl)
+  -- Because the hypothesis is only applied to positive variables,
+  -- which are always possible-lane (see `InductionDescriptor`),
+  -- we can ignore the lane type here.
+  (_: SingleLaneVarType)
   (x: Nat)
 :
-  PairExpr
+  SingleLanePairExpr
 :=
-  desc.foldr (InductionDescriptor.hypothesis x) (.var x)
+  desc.foldr (InductionDescriptor.hypothesis x) (.var .posLane x)
 
 def MutCoindDescriptor.hypothesis
   (desc: MutCoindDescriptor dl)
+  -- We can ignore the lane analogously to `MutIndDescriptor.hypothesis`.
+  (_: SingleLaneVarType)
   (x: Nat)
 :
-  PairExpr
+  SingleLanePairExpr
 :=
-  desc.foldr (CoinductionDescriptor.hypothesis x) (.var x)
+  desc.foldr (CoinductionDescriptor.hypothesis x) (.var .defLane x)
 
 def MutIndDescriptor.hypothesify
   (desc: MutIndDescriptor dl)
-  (expr: PairExpr)
+  (expr: SingleLanePairExpr)
 :
-  PairExpr
+  SingleLanePairExpr
 :=
   expr.replacePosVars desc.hypothesis
 
 def MutCoindDescriptor.hypothesify
   (desc: MutCoindDescriptor dl)
-  (expr: PairExpr)
+  (expr: SingleLanePairExpr)
 :
-  PairExpr
+  SingleLanePairExpr
 :=
-  .cpl (expr.replacePosVars desc.hypothesis)
+  .compl (expr.replacePosVars desc.hypothesis)
 
 def InductionDescriptor.exprLeft
   (desc: InductionDescriptor dl)
 :
-  PairExpr
+  SingleLanePairExpr
 :=
-  .var desc.left
+  .var .posLane desc.left
 
 def CoinductionDescriptor.exprLeft
   (desc: CoinductionDescriptor dl)
 :
-  PairExpr
+  SingleLanePairExpr
 :=
   desc.left
 
 def InductionDescriptor.exprRite
   (desc: InductionDescriptor dl)
 :
-  PairExpr
+  SingleLanePairExpr
 :=
   desc.rite
 
 def CoinductionDescriptor.exprRite
   (desc: CoinductionDescriptor dl)
 :
-  PairExpr
+  SingleLanePairExpr
 :=
-  .cpl (.var desc.rite)
+  .compl (.var .defLane desc.rite)
 
 inductive Subset
   (dl: PairDl)
 :
-  PairExpr → PairExpr → Type
+  SingleLanePairExpr → SingleLanePairExpr → Type
 
-| null: Subset dl .null .null
+| null: Subset dl null null
 | pair
     (sl: Subset dl al bl)
     (sr: Subset dl ar br)
   :
-    Subset dl (.pair al ar) (.pair bl br)
-| unL (s: Subset dl a b) {r: PairExpr}: Subset dl a (.un b r)
-| unR (s: Subset dl a b) {l: PairExpr}: Subset dl a (.un l b)
+    Subset dl (pair al ar) (pair bl br)
+| unL (s: Subset dl a b) {r: SingleLanePairExpr}: Subset dl a (un b r)
+| unR (s: Subset dl a b) {l: SingleLanePairExpr}: Subset dl a (un l b)
 | mutInduction
     (desc: MutIndDescriptor dl)
     (premises:
       (i: desc.Index) →
-      Subset dl (desc.hypothesify desc[i].expansion) desc[i].rite)
+      Subset
+        dl
+        (desc.hypothesify (desc[i].expansion.toLane .posLane))
+        desc[i].rite)
     (i: desc.Index)
   :
     Subset dl desc[i].exprLeft desc[i].exprRite
@@ -168,7 +179,10 @@ inductive Subset
     (desc: MutCoindDescriptor dl)
     (premises:
       (i: desc.Index) →
-      Subset dl desc[i].left (desc.hypothesify desc[i].expansion))
+      Subset
+        dl
+        desc[i].left
+        (desc.hypothesify (desc[i].expansion.toLane .defLane)))
     (i: desc.Index)
   :
     Subset dl desc[i].exprLeft desc[i].exprRite
@@ -179,16 +193,15 @@ def Subset.induction
   (premise:
     Subset
       dl
-      (desc.expansion.replacePosVars fun x =>
-        desc.hypothesis x (.var x))
+      ((desc.expansion.toLane .posLane).replacePosVars fun _ x =>
+        desc.hypothesis x (.var .posLane x))
       desc.rite)
 :
-  Subset dl (.var desc.left) desc.rite
+  Subset dl (.var .posLane desc.left) desc.rite
 :=
   Subset.mutInduction
     [desc]
-    (fun
-      | ⟨0, _⟩ => premise)
+    (fun | ⟨0, _⟩ => premise)
     ⟨0, Nat.zero_lt_succ _⟩
 
 def Subset.coinduction
@@ -197,16 +210,15 @@ def Subset.coinduction
     Subset
       dl
       desc.left
-      (.cpl
-        (desc.expansion.replacePosVars fun x =>
-          desc.hypothesis x (.var x))))
+      (.compl
+        ((desc.expansion.toLane .defLane).replacePosVars fun _ x =>
+          desc.hypothesis x (.var .defLane x))))
 :
-  Subset dl desc.left (.cpl (.var desc.rite))
+  Subset dl desc.left (.compl (.var .defLane desc.rite))
 :=
   Subset.mutCoinduction
     [desc]
-    (fun
-      | ⟨0, _⟩ => premise)
+    (fun | ⟨0, _⟩ => premise)
     ⟨0, Nat.zero_lt_succ _⟩
 
 
@@ -216,11 +228,11 @@ def Subset.simpleInduction
   (premise:
     Subset
       dl
-      ((dl.getDef left).replacePosVars fun x =>
-        if left = x then PairExpr.ir rite (.var x) else (.var x))
+      (((dl.getDef left).toLane .posLane).replacePosVars fun _ x =>
+        if left = x then PairExpr.ir rite (.var .posLane x) else (.var .posLane x))
       rite)
 :
-  Subset dl (.var left) rite
+  Subset dl (.var .posLane left) rite
 :=
   Subset.induction
     {
@@ -239,11 +251,11 @@ def Subset.simpleCoinduction
     Subset
       dl
       left
-      (.cpl
-        ((dl.getDef rite).replacePosVars fun x =>
-          if rite = x then PairExpr.ir (.cpl left) (.var x) else (.var x))))
+      (.compl
+        (((dl.getDef rite).toLane .defLane).replacePosVars fun _ x =>
+          if rite = x then PairExpr.ir (.compl left) (.var .defLane x) else (.var .defLane x))))
 :
-  Subset dl left (.cpl (.var rite))
+  Subset dl left (.compl (.var .defLane rite))
 :=
   Subset.coinduction
     {
