Etst/WFC/Utils/Expr.lean
@@ -1,0 +1,92 @@
+import Etst.WFC.Ch2_Interpretation
+
+namespace Etst
+
+
+namespace SingleLaneExpr
+  def var (lane: SingleLaneVarType) (x: Nat): SingleLaneExpr sig :=
+    Expr.var lane x
+  def bvar (x: Nat): SingleLaneExpr sig :=
+    Expr.bvar x
+  def op
+    (opr: sig.Op)
+    (args: (param: sig.Params opr) → SingleLaneExpr sig)
+  :
+    SingleLaneExpr sig
+  :=
+    Expr.op opr args
+  def compl (body: SingleLaneExpr sig): SingleLaneExpr sig :=
+    Expr.compl body
+  def arbUn (body: SingleLaneExpr sig): SingleLaneExpr sig :=
+    Expr.arbUn body
+  def arbIr (body: SingleLaneExpr sig): SingleLaneExpr sig :=
+    Expr.arbIr body
+end SingleLaneExpr
+
+/-
+  This proposition asserts that the "context" part of an expression
+  (anything not under a complement) only refers to variables from
+  the given lane.
+-/
+inductive Expr.LaneEqCtx (lane: SingleLaneVarType): Expr E sig → Prop
+| var (x: Nat): Expr.LaneEqCtx lane (Expr.var lane x)
+| bvar (x: Nat): Expr.LaneEqCtx lane (Expr.bvar x)
+| op
+    (opr: sig.Op)
+    (args: (param: sig.Params opr) → Expr E sig)
+    (argsLaneEq: (param: sig.Params opr) → Expr.LaneEqCtx lane (args param))
+  :
+    Expr.LaneEqCtx lane (Expr.op opr args)
+| compl (body: Expr E sig): Expr.LaneEqCtx lane (body.compl)
+| arbUn
+    (laneEqBody: Expr.LaneEqCtx lane body)
+  :
+    Expr.LaneEqCtx lane (Expr.arbUn body)
+| arbIr
+    (laneEqBody: Expr.LaneEqCtx lane body)
+  :
+    Expr.LaneEqCtx lane (Expr.arbIr body)
+
+def Expr.LaneEqCtx.elimOp
+  {sig: Signature}
+  {opr: sig.Op}
+  {args: (param: sig.Params opr) → Expr E sig}
+  (laneEq: Expr.LaneEqCtx lane (Expr.op opr args))
+  (param: sig.Params opr)
+:
+  Expr.LaneEqCtx lane (args param)
+:=
+  match laneEq with
+  | .op _ _ argsLaneEq => argsLaneEq param
+
+def Expr.LaneEqCtx.elimArbUn
+  (laneEq: Expr.LaneEqCtx lane (body.arbUn))
+:
+  Expr.LaneEqCtx lane body
+:=
+  match laneEq with
+  | .arbUn laneEqBody => laneEqBody
+
+def Expr.LaneEqCtx.elimArbIr
+  (laneEq: Expr.LaneEqCtx lane (body.arbIr))
+:
+  Expr.LaneEqCtx lane body
+:=
+  match laneEq with
+  | .arbIr laneEqBody => laneEqBody
+
+
+def BasicExpr.posLaneEqCtx
+  (expr: BasicExpr sig)
+  (lane: SingleLaneVarType)
+:
+  Expr.LaneEqCtx lane (expr.toLane lane)
+:=
+  match expr with
+  | .var x => .var x
+  | .bvar x => .bvar x
+  | .op opr args =>
+    .op opr _ (fun param => (args param).posLaneEqCtx lane)
+  | .compl body => .compl (body.toLane lane.toggle)
+  | .arbUn body => .arbUn (body.posLaneEqCtx lane)
+  | .arbIr body => .arbIr (body.posLaneEqCtx lane)
