Etst/WFC/Utils/InterpretationMono.lean
@@ -1,0 +1,441 @@
+/-
+  In this file, we prove monotonicity of the interpretation of Expr
+  constructors. Unlike the file `Interpretation.lean`, where the assumptions
+  are that the valuations are ordered, here we assume that the interpretations
+  of the sub-expressions are ordered.
+-/
+import Etst.WFC.Utils.PairExpr
+
+namespace Etst
+
+
+namespace SingleLaneExpr
+  def inter_mono_std_op
+    {salg: Salgebra sig}
+    {bv0 bv1: List salg.D}
+    {b0 c0 b1 c1: Valuation salg.D}
+    (le:
+      ∀ param: sig.Params o,
+        Set.Subset
+          ((args0 param).interpretation salg bv0 b0 c0)
+          ((args1 param).interpretation salg bv1 b1 c1))
+  :
+    Set.Subset
+      ((op o args0).interpretation salg bv0 b0 c0)
+      ((op o args1).interpretation salg bv1 b1 c1)
+  :=
+    fun _ dIn => salg.isMonotonic o _ _ le dIn
+  
+  def eq_op_of_eq
+    {salg: Salgebra sig}
+    {bv0 bv1: List salg.D}
+    {b0 c0 b1 c1: Valuation salg.D}
+    (eq:
+      ∀ param: sig.Params o,
+      Eq
+        ((args0 param).interpretation salg bv0 b0 c0)
+        ((args1 param).interpretation salg bv1 b1 c1))
+  :
+    Eq
+      ((op o args0).interpretation salg bv0 b0 c0)
+      ((op o args1).interpretation salg bv1 b1 c1)
+  :=
+    le_antisymm
+      (inter_mono_std_op (fun param => le_of_eq (eq param)))
+      (inter_mono_std_op (fun param => le_of_eq (eq param).symm))
+  
+  
+  -- Note we're using `b0 b0` and `b1 b1` in the assumption.
+  def inter_mono_std_compl
+    {salg: Salgebra sig}
+    {bv0 bv1: List salg.D}
+    {b0 b1: Valuation salg.D}
+    (c0 c1: Valuation salg.D)
+    (le:
+      Set.Subset
+        (e1.interpretation salg bv1 b1 b1)
+        (e0.interpretation salg bv0 b0 b0))
+  :
+    Set.Subset
+      ((compl e0).interpretation salg bv0 b0 c0)
+      ((compl e1).interpretation salg bv1 b1 c1)
+  :=
+    fun _ ins =>
+      inCompl c0 (fun isPos => inComplElim ins (le isPos))
+  
+  def eq_compl_of_eq
+    {salg: Salgebra sig}
+    {bv0 bv1: List salg.D}
+    {b0 b1: Valuation salg.D}
+    (c0 c1: Valuation salg.D)
+    (eq:
+      Eq
+        (e0.interpretation salg bv0 b0 b0)
+        (e1.interpretation salg bv1 b1 b1))
+  :
+    Eq
+      ((compl e0).interpretation salg bv0 b0 c0)
+      ((compl e1).interpretation salg bv1 b1 c1)
+  :=
+    le_antisymm
+      (inter_mono_std_compl c0 c1 (le_of_eq eq.symm))
+      (inter_mono_std_compl c0 c1 (le_of_eq eq))
+  
+  
+  def inter_mono_std_arbUn
+    {salg: Salgebra sig}
+    {bv0 bv1: List salg.D}
+    {b0 c0 b1 c1: Valuation salg.D}
+    (le:
+      ∀ dB,
+      Set.Subset
+        (e0.interpretation salg (dB :: bv0) b0 c0)
+        (e1.interpretation salg (dB :: bv1) b1 c1))
+  :
+    Set.Subset
+      ((arbUn e0).interpretation salg bv0 b0 c0)
+      ((arbUn e1).interpretation salg bv1 b1 c1)
+  :=
+    fun _ ⟨dB, isDef⟩ => ⟨dB, (le dB) isDef⟩
+  
+  def eq_arbUn_of_eq
+    {salg: Salgebra sig}
+    {bv0 bv1: List salg.D}
+    {b0 c0 b1 c1: Valuation salg.D}
+    (eq:
+      ∀ dB,
+      Eq
+        (e0.interpretation salg (dB :: bv0) b0 c0)
+        (e1.interpretation salg (dB :: bv1) b1 c1))
+  :
+    Eq
+      ((arbUn e0).interpretation salg bv0 b0 c0)
+      ((arbUn e1).interpretation salg bv1 b1 c1)
+  :=
+    le_antisymm
+      (inter_mono_std_arbUn (fun dB => le_of_eq (eq dB)))
+      (inter_mono_std_arbUn (fun dB => le_of_eq (eq dB).symm))
+  
+  
+  def inter_mono_std_arbIr
+    {salg: Salgebra sig}
+    {bv0 bv1: List salg.D}
+    {b0 c0 b1 c1: Valuation salg.D}
+    (le:
+      ∀ dB,
+      Set.Subset
+        (e0.interpretation salg (dB :: bv0) b0 c0)
+        (e1.interpretation salg (dB :: bv1) b1 c1))
+  :
+    Set.Subset
+      ((arbIr e0).interpretation salg bv0 b0 c0)
+      ((arbIr e1).interpretation salg bv1 b1 c1)
+  :=
+    fun _ h dB => (le dB) (h dB)
+  
+  def eq_arbIr_of_eq
+    {salg: Salgebra sig}
+    {bv0 bv1: List salg.D}
+    {b0 c0 b1 c1: Valuation salg.D}
+    (eq:
+      ∀ dB,
+      Eq
+        (e0.interpretation salg (dB :: bv0) b0 c0)
+        (e1.interpretation salg (dB :: bv1) b1 c1))
+  :
+    Eq
+      ((arbIr e0).interpretation salg bv0 b0 c0)
+      ((arbIr e1).interpretation salg bv1 b1 c1)
+  :=
+    le_antisymm
+      (inter_mono_std_arbIr (fun dB => le_of_eq (eq dB)))
+      (inter_mono_std_arbIr (fun dB => le_of_eq (eq dB).symm))
+  
+end SingleLaneExpr
+
+namespace BasicExpr
+  open PairExpr
+  open SingleLaneExpr
+  
+  def triIntp2_mono_std_compl
+    (c0 c1: Valuation Pair)
+    (le: triIntp2 e1 bv1 b1 b1 ≤ triIntp2 e0 bv0 b0 b0)
+  :
+    triIntp2 (compl e0) bv0 b0 c0 ≤ triIntp2 (compl e1) bv1 b1 c1
+  := {
+    defLe := inter_mono_std_compl c0 c1 le.posLe
+    posLe := inter_mono_std_compl c0 c1 le.defLe
+  }
+
+  def eq_triIntp2_compl_of_eq
+    (c0 c1: Valuation Pair)
+    (eq: triIntp2 e0 bv0 b0 b0 = triIntp2 e1 bv1 b1 b1)
+  :
+    triIntp2 (compl e0) bv0 b0 c0 = triIntp2 (compl e1) bv1 b1 c1
+  :=
+    Set3.eq
+      (eq_compl_of_eq c0 c1 (Set3.pos_eq eq))
+      (eq_compl_of_eq c0 c1 (Set3.def_eq eq))
+  
+  
+  def triIntp2_mono_std_arbUn
+    (le:
+      ∀ dB,
+      triIntp2 e0 (dB :: bv0) b0 c0 ≤ triIntp2 e1 (dB :: bv1) b1 c1)
+  :
+    triIntp2 (arbUn e0) bv0 b0 c0 ≤ triIntp2 (arbUn e1) bv1 b1 c1
+  := {
+    defLe := inter_mono_std_arbUn (fun (dB: Pair) => (le dB).defLe)
+    posLe := inter_mono_std_arbUn (fun (dB: Pair) => (le dB).posLe)
+  }
+  
+  def eq_triIntp2_arbUn_of_eq
+    (eq:
+      ∀ dB,
+      triIntp2 e0 (dB :: bv0) b0 c0 = triIntp2 e1 (dB :: bv1) b1 c1)
+  :
+    triIntp2 (arbUn e0) bv0 b0 c0 = triIntp2 (arbUn e1) bv1 b1 c1
+  :=
+    Set3.eq
+      (eq_arbUn_of_eq (fun (dB: Pair) => Set3.def_eq (eq dB)))
+      (eq_arbUn_of_eq (fun (dB: Pair) => Set3.pos_eq (eq dB)))
+  
+  
+  def triIntp2_mono_std_arbIr
+    (le:
+      ∀ dB,
+      triIntp2 e0 (dB :: bv0) b0 c0 ≤ triIntp2 e1 (dB :: bv1) b1 c1)
+  :
+    triIntp2 (arbIr e0) bv0 b0 c0 ≤ triIntp2 (arbIr e1) bv1 b1 c1
+  := {
+    defLe := inter_mono_std_arbIr (fun (dB: Pair) => (le dB).defLe)
+    posLe := inter_mono_std_arbIr (fun (dB: Pair) => (le dB).posLe)
+  }
+  
+  def eq_triIntp2_arbIr_of_eq
+    (eq:
+      ∀ dB,
+      triIntp2 e0 (dB :: bv0) b0 c0 = triIntp2 e1 (dB :: bv1) b1 c1)
+  :
+    triIntp2 (arbIr e0) bv0 b0 c0 = triIntp2 (arbIr e1) bv1 b1 c1
+  :=
+    Set3.eq
+      (eq_arbIr_of_eq (fun (dB: Pair) => Set3.def_eq (eq dB)))
+      (eq_arbIr_of_eq (fun (dB: Pair) => Set3.pos_eq (eq dB)))
+
+end BasicExpr
+
+
+namespace SingleLaneExpr
+  open PairExpr
+  
+  def intp2_mono_std_pair
+    {l0 l1 r0 r1: SingleLanePairExpr}
+    (leL: intp2 l0 bv0 b0 c0 ≤ intp2 l1 bv1 b1 c1)
+    (leR: intp2 r0 bv0 b0 c0 ≤ intp2 r1 bv1 b1 c1)
+  :
+    intp2 (pair l0 r0) bv0 b0 c0 ⊆ intp2 (pair l1 r1) bv1 b1 c1
+  :=
+    fun
+    | .pair _ _, isDef =>
+      let ⟨insL, insR⟩ := inPairElim isDef
+      inPair (leL insL) (leR insR)
+  
+  def eq_intp2_pair_of_eq
+    (eqL: intp2 l0 bv0 b0 c0 = intp2 l1 bv1 b1 c1)
+    (eqR: intp2 r0 bv0 b0 c0 = intp2 r1 bv1 b1 c1)
+  :
+    intp2 (pair l0 r0) bv0 b0 c0 = intp2 (pair l1 r1) bv1 b1 c1
+  :=
+    le_antisymm
+      (intp2_mono_std_pair (le_of_eq eqL) (le_of_eq eqR))
+      (intp2_mono_std_pair (le_of_eq eqL.symm) (le_of_eq eqR.symm))
+  
+  
+  def intp2_mono_std_un
+    (leL: intp2 l0 bv0 b0 c0 ≤ intp2 l1 bv1 b1 c1)
+    (leR: intp2 r0 bv0 b0 c0 ≤ intp2 r1 bv1 b1 c1)
+  :
+    intp2 (un l0 r0) bv0 b0 c0 ⊆ intp2 (un l1 r1) bv1 b1 c1
+  :=
+    fun _ ins =>
+      (inUnElim ins).elim
+        (fun insL => inUnL (leL insL))
+        (fun insR => inUnR (leR insR))
+  
+  def eq_intp2_un_of_eq
+    (eqL: intp2 l0 bv0 b0 c0 = intp2 l1 bv1 b1 c1)
+    (eqR: intp2 r0 bv0 b0 c0 = intp2 r1 bv1 b1 c1)
+  :
+    intp2 (un l0 r0) bv0 b0 c0 = intp2 (un l1 r1) bv1 b1 c1
+  :=
+    le_antisymm
+      (intp2_mono_std_un (le_of_eq eqL) (le_of_eq eqR))
+      (intp2_mono_std_un (le_of_eq eqL.symm) (le_of_eq eqR.symm))
+  
+  
+  def intp2_mono_std_ir
+    (leL: intp2 l0 bv0 b0 c0 ≤ intp2 l1 bv1 b1 c1)
+    (leR: intp2 r0 bv0 b0 c0 ≤ intp2 r1 bv1 b1 c1)
+  :
+    intp2 (ir l0 r0) bv0 b0 c0 ⊆ intp2 (ir l1 r1) bv1 b1 c1
+  :=
+    fun _ ins =>
+      let ⟨insL, insR⟩ := inIrElim ins
+      inIr (leL insL) (leR insR)
+  
+  def eq_intp2_ir_of_eq
+    (eqL: intp2 l0 bv0 b0 c0 = intp2 l1 bv1 b1 c1)
+    (eqR: intp2 r0 bv0 b0 c0 = intp2 r1 bv1 b1 c1)
+  :
+    intp2 (ir l0 r0) bv0 b0 c0 = intp2 (ir l1 r1) bv1 b1 c1
+  :=
+    le_antisymm
+      (intp2_mono_std_ir (le_of_eq eqL) (le_of_eq eqR))
+      (intp2_mono_std_ir (le_of_eq eqL.symm) (le_of_eq eqR.symm))
+  
+  
+  def intp2_mono_std_condSome
+    (le: intp2 e0 bv0 b0 c0 ≤ intp2 e1 bv1 b1 c1)
+  :
+    intp2 (condSome e0) bv0 b0 c0 ⊆ intp2 (condSome e1) bv1 b1 c1
+  :=
+    fun _ ins =>
+      let ⟨_, insE⟩ := inCondSomeElim ins (d := .null)
+      inCondSome (le insE) .null
+  
+  def eq_intp2_condSome_of_eq
+    (eq: intp2 e0 bv0 b0 c0 = intp2 e1 bv1 b1 c1)
+  :
+    intp2 (condSome e0) bv0 b0 c0 = intp2 (condSome e1) bv1 b1 c1
+  :=
+    le_antisymm
+      (intp2_mono_std_condSome (le_of_eq eq))
+      (intp2_mono_std_condSome (le_of_eq eq.symm))
+  
+  
+  def intp2_mono_std_condFull
+    (le: intp2 e0 bv0 b0 c0 ≤ intp2 e1 bv1 b1 c1)
+  :
+    intp2 (condFull e0) bv0 b0 c0 ⊆ intp2 (condFull e1) bv1 b1 c1
+  :=
+    fun _ ins =>
+      let insE := inCondFullElim ins (d := .null)
+      inCondFull (fun d => le (insE d)) .null
+  
+  def eq_intp2_condFull_of_eq
+    (eq: intp2 e0 bv0 b0 c0 = intp2 e1 bv1 b1 c1)
+  :
+    intp2 (condFull e0) bv0 b0 c0 = intp2 (condFull e1) bv1 b1 c1
+  :=
+    le_antisymm
+      (intp2_mono_std_condFull (le_of_eq eq))
+      (intp2_mono_std_condFull (le_of_eq eq.symm))
+  
+end SingleLaneExpr
+
+namespace BasicExpr
+  open PairExpr
+  open SingleLaneExpr
+  
+  def triIntp2_mono_std_pair
+    (leL: triIntp2 l0 bv0 b0 c0 ≤ triIntp2 l1 bv1 b1 c1)
+    (leR: triIntp2 r0 bv0 b0 c0 ≤ triIntp2 r1 bv1 b1 c1)
+  :
+    triIntp2 (pair l0 r0) bv0 b0 c0 ≤ triIntp2 (pair l1 r1) bv1 b1 c1
+  := {
+    defLe := intp2_mono_std_pair leL.defLe leR.defLe
+    posLe := intp2_mono_std_pair leL.posLe leR.posLe
+  }
+  
+  def eq_triIntp2_pair_of_eq
+    (eqL: triIntp2 l0 bv0 b0 c0 = triIntp2 l1 bv1 b1 c1)
+    (eqR: triIntp2 r0 bv0 b0 c0 = triIntp2 r1 bv1 b1 c1)
+  :
+    triIntp2 (pair l0 r0) bv0 b0 c0 = triIntp2 (pair l1 r1) bv1 b1 c1
+  :=
+    Set3.eq
+      (eq_intp2_pair_of_eq (Set3.def_eq eqL) (Set3.def_eq eqR))
+      (eq_intp2_pair_of_eq (Set3.pos_eq eqL) (Set3.pos_eq eqR))
+  
+  
+  def triIntp2_mono_std_un
+    (leL: triIntp2 l0 bv0 b0 c0 ≤ triIntp2 l1 bv1 b1 c1)
+    (leR: triIntp2 r0 bv0 b0 c0 ≤ triIntp2 r1 bv1 b1 c1)
+  :
+    triIntp2 (un l0 r0) bv0 b0 c0 ≤ triIntp2 (un l1 r1) bv1 b1 c1
+  := {
+    defLe := intp2_mono_std_un leL.defLe leR.defLe
+    posLe := intp2_mono_std_un leL.posLe leR.posLe
+  }
+  
+  def eq_triIntp2_un_of_eq
+    (eqL: triIntp2 l0 bv0 b0 c0 = triIntp2 l1 bv1 b1 c1)
+    (eqR: triIntp2 r0 bv0 b0 c0 = triIntp2 r1 bv1 b1 c1)
+  :
+    triIntp2 (un l0 r0) bv0 b0 c0 = triIntp2 (un l1 r1) bv1 b1 c1
+  :=
+    Set3.eq
+      (eq_intp2_un_of_eq (Set3.def_eq eqL) (Set3.def_eq eqR))
+      (eq_intp2_un_of_eq (Set3.pos_eq eqL) (Set3.pos_eq eqR))
+  
+  
+  def triIntp2_mono_std_ir
+    (leL: triIntp2 l0 bv0 b0 c0 ≤ triIntp2 l1 bv1 b1 c1)
+    (leR: triIntp2 r0 bv0 b0 c0 ≤ triIntp2 r1 bv1 b1 c1)
+  :
+    triIntp2 (ir l0 r0) bv0 b0 c0 ≤ triIntp2 (ir l1 r1) bv1 b1 c1
+  := {
+    defLe := intp2_mono_std_ir leL.defLe leR.defLe
+    posLe := intp2_mono_std_ir leL.posLe leR.posLe
+  }
+  
+  def eq_triIntp2_ir_of_eq
+    (eqL: triIntp2 l0 bv0 b0 c0 = triIntp2 l1 bv1 b1 c1)
+    (eqR: triIntp2 r0 bv0 b0 c0 = triIntp2 r1 bv1 b1 c1)
+  :
+    triIntp2 (ir l0 r0) bv0 b0 c0 = triIntp2 (ir l1 r1) bv1 b1 c1
+  :=
+    Set3.eq
+      (eq_intp2_ir_of_eq (Set3.def_eq eqL) (Set3.def_eq eqR))
+      (eq_intp2_ir_of_eq (Set3.pos_eq eqL) (Set3.pos_eq eqR))
+  
+  
+  def triIntp2_mono_std_condSome
+    (le: triIntp2 e0 bv0 b0 c0 ≤ triIntp2 e1 bv1 b1 c1)
+  :
+    triIntp2 (condSome e0) bv0 b0 c0 ≤ triIntp2 (condSome e1) bv1 b1 c1
+  := {
+    defLe := intp2_mono_std_condSome le.defLe
+    posLe := intp2_mono_std_condSome le.posLe
+  }
+  
+  def eq_triIntp2_condSome_of_eq
+    (eq: triIntp2 e0 bv0 b0 c0 = triIntp2 e1 bv1 b1 c1)
+  :
+    triIntp2 (condSome e0) bv0 b0 c0 = triIntp2 (condSome e1) bv1 b1 c1
+  :=
+    Set3.eq
+      (eq_intp2_condSome_of_eq (Set3.def_eq eq))
+      (eq_intp2_condSome_of_eq (Set3.pos_eq eq))
+  
+  
+  def triIntp2_mono_std_condFull
+    (le: triIntp2 e0 bv0 b0 c0 ≤ triIntp2 e1 bv1 b1 c1)
+  :
+    triIntp2 (condFull e0) bv0 b0 c0 ≤ triIntp2 (condFull e1) bv1 b1 c1
+  := {
+    defLe := intp2_mono_std_condFull le.defLe
+    posLe := intp2_mono_std_condFull le.posLe
+  }
+  
+  def eq_triIntp2_condFull_of_eq
+    (eq: triIntp2 e0 bv0 b0 c0 = triIntp2 e1 bv1 b1 c1)
+  :
+    triIntp2 (condFull e0) bv0 b0 c0 = triIntp2 (condFull e1) bv1 b1 c1
+  :=
+    Set3.eq
+      (eq_intp2_condFull_of_eq (Set3.def_eq eq))
+      (eq_intp2_condFull_of_eq (Set3.pos_eq eq))
+  
+end BasicExpr
