Etst/WFC/Utils/Set3.lean
@@ -181,7 +181,7 @@ namespace Set3
     defLePos := fun _ dIn d => (dIn d).toPos
   }
   
-  def cpl (s: Set3 D): Set3 D := {
+  def compl (s: Set3 D): Set3 D := {
     defMem := fun d => d ∉ s.posMem
     posMem := fun d => d ∉ s.defMem
     defLePos := fun _ => notDefOfNotPos
@@ -199,17 +199,17 @@ namespace Set3
     defLePos := fun _d ddIn dd => (ddIn dd).toPos
   }
   
-  def cpl_inj_eq
-    (eq: cpl s0 = cpl s1)
+  def compl_inj_eq
+    (eq: compl s0 = compl s1)
   :
     s0 = s1
   :=
-    let defEq: s0.cpl.defMem = s1.cpl.defMem := congr rfl eq
-    let posEq: s0.cpl.posMem = s1.cpl.posMem := congr rfl eq
+    let defEq: s0.compl.defMem = s1.compl.defMem := congr rfl eq
+    let posEq: s0.compl.posMem = s1.compl.posMem := congr rfl eq
     Set3.eq (compl_inj_iff.mp posEq) (compl_inj_iff.mp defEq)
   
-  def cpl_inj_neq (neq: s0 ≠ s1): cpl s0 ≠ cpl s1 :=
-    cpl_inj_eq.mt neq
+  def compl_inj_neq (neq: s0 ≠ s1): compl s0 ≠ compl s1 :=
+    compl_inj_eq.mt neq
   
   
   instance unionInst (D: Type u): Union (Set3 D) where
@@ -468,11 +468,11 @@ namespace Set3
   :=
     compl_le_compl (posLe ab)
   
-  def LeStd.compl_le_compl (ab: LeStd a b): b.cpl ≤ a.cpl :=
+  def LeStd.compl_le_compl (ab: LeStd a b): b.compl ≤ a.compl :=
     LeStd.mk (LeStd.notPosLe ab) (LeStd.notDefLe ab)
   
-  def LtStd.compl_lt_compl (ab: LtStd a b): b.cpl < a.cpl :=
-    LtStd.mk ab.toLe.notPosLe ab.toLe.notDefLe (cpl_inj_neq ab.neq.symm)
+  def LtStd.compl_lt_compl (ab: LtStd a b): b.compl < a.compl :=
+    LtStd.mk ab.toLe.notPosLe ab.toLe.notDefLe (compl_inj_neq ab.neq.symm)
   
   
   -- The standard order is antisymmetric.
